The number of normal forms is preserved trhough isopres

theories/enumnf.v
@@ -38,16 +38,16 @@ Definition normal_sz (n : nat) u :=
   [&& size u == n, u \in words_of P & normal (prelat P) u].
 Definition enum_normal_next norf :=
   [seq x <- [seq g :: w | g <- pgen P, w <- norf] | ~~ rew1 x].
-Definition enum_normal n := iter n enum_normal_next [:: [::]].
+Definition enum_normal_sz n := iter n enum_normal_next [:: [::]].
 
 Lemma normal_sz0 : normal_sz 0 [::].
 Proof. by rewrite /normal_sz /=; apply normal0; case: convP. Qed.
 
-Lemma normal_sz_enum_normal n : all (normal_sz n) (enum_normal n).
+Lemma normal_sz_enum_normal_sz n : all (normal_sz n) (enum_normal_sz n).
 Proof.
 elim: n => [| n]; first by rewrite /= normal_sz0.
-rewrite {2}/enum_normal /= -/(enum_normal n).
-move: (enum_normal n) => norf /allP /= allnorf; apply/allP => /= [[| u0 u]].
+rewrite {2}/enum_normal_sz /= -/(enum_normal_sz n).
+move: (enum_normal_sz n) => norf /allP /= allnorf; apply/allP => /= [[| u0 u]].
   by rewrite mem_filter => /andP[_ /allpairsP[[/= u0 u []]]].
 rewrite mem_filter => /andP[]; case: rew1P => nrew // _.
 case/allpairsP => /= - [v0 v]/= [ugen unor []] equ0 equ; subst v0 v.
@@ -58,12 +58,12 @@ have -> : (u0 :: u \in words_of P) = (u \in words_of P).
 by case: (u \in _).
 Qed.
 
-Lemma count_mem_enum_normal n u :
-  normal_sz n u -> count_mem u (enum_normal n) = 1%N.
+Lemma count_mem_enum_normal_sz n u :
+  normal_sz n u -> count_mem u (enum_normal_sz n) = 1%N.
 Proof.
 elim: n u => [|n]; first by case.
-rewrite {2}/enum_normal /= -/(enum_normal n).
-move: (enum_normal n) => norf Hn [|u0 u] //=.
+rewrite {2}/enum_normal_sz /= -/(enum_normal_sz n).
+move: (enum_normal_sz n) => norf Hn [|u0 u] //=.
 rewrite /normal_sz /= eqSS.
 have -> : (u0 :: u \in words_of P) = (u0 \in pgen P) && (u \in words_of P).
   by rewrite !unfold_in /words_of /=.
@@ -83,20 +83,149 @@ case: rew1P => //= v; rewrite rew0 /= => /mapP[/= w + _].
 by case/and3P: unorf => _ _ /eqP ->.
 Qed.
 
-Lemma uniq_enum_normal n : uniq (enum_normal n).
+Lemma uniq_enum_normal_sz n : uniq (enum_normal_sz n).
 Proof.
-have /allP /= allnorf := normal_sz_enum_normal n.
+have /allP /= allnorf := normal_sz_enum_normal_sz n.
 apply: count_mem_uniq => /= u.
-case: (boolP (u \in _)) => [/allnorf/count_mem_enum_normal -> // | /= unotin].
+case: (boolP (u \in _)) => [/allnorf/count_mem_enum_normal_sz -> // | /= unotin].
 exact/count_memPn.
 Qed.
 
-Lemma mem_enum_normalP n u : (u \in enum_normal n) = normal_sz n u.
+Lemma mem_enum_normalP n u : (u \in enum_normal_sz n) = normal_sz n u.
 Proof.
-have /allP /= allnorf := normal_sz_enum_normal n.
+have /allP /= allnorf := normal_sz_enum_normal_sz n.
 case: (boolP (u \in _)) => [/allnorf -> // | /= unotin].
-apply/esym; apply/contraNF: unotin => /count_mem_enum_normal.
+apply/esym; apply/contraNF: unotin => /count_mem_enum_normal_sz.
 by rewrite -has_pred1 has_count => ->.
 Qed.
 
+Lemma enum_normalE n :
+  enum_normal_sz n = [::] ->
+  forall u,
+    (u \in words_of P) && (normal (prelat P) u) =
+      (u \in flatten (traject enum_normal_next [:: [::]] n)).
+Proof.
+move=> Hiter u.
+have gt m : m >= n -> enum_normal_sz m = [::].
+  elim: m => [|m IHm] /=.
+    by rewrite leqn0 => /eqP Hn; rewrite Hn /= in Hiter.
+  rewrite leq_eqVlt ltnS => /orP[/eqP eq| /IHm ->].
+    by move: Hiter; rewrite eq /=.
+  by rewrite /enum_normal_next /=; elim: (pgen P).
+apply/idP/idP.
+  case/andP => uin noru.
+  have {uin}noru : normal_sz (size u) u by rewrite /normal_sz eqxx uin noru.
+  apply/flattenP => /=; exists (iter (size u) enum_normal_next [:: [::]]).
+    apply/trajectP; exists (size u) => //.
+    apply/negP => /negP; rewrite -leqNgt => {}/gt eqnor.
+    by rewrite -mem_enum_normalP eqnor in noru.
+  by rewrite mem_enum_normalP.
+case/flattenP => /= l /trajectP[m ltmn {l}->].
+by rewrite mem_enum_normalP => /and3P[_ -> ->].
+Qed.
+
+(** Given a bound returns the list of normal forms of size less than bound
+and a boolean telling if that list is complete *)
+Definition enum_normal bound :=
+  let l := traject enum_normal_next [:: [::]] bound in
+  (flatten l, last [::[::]] l == [::]).
+Definition is_enum_normal l :=
+  uniq l /\ forall u, (u \in words_of P) && (normal (prelat P) u) = (u \in l).
+
+Lemma enum_normalP bound :
+  let: (l, ok) := enum_normal bound in ok -> is_enum_normal l.
+Proof.
+move => /= H; split; first last.
+  rewrite /enum_normal; case: bound H => [//| b].
+  rewrite {2}trajectSr /= last_traject => /eqP/[dup]/enum_normalE H ->.
+  by rewrite flatten_rcons cats0.
+elim: bound {H} => // n IHn.
+rewrite trajectSr flatten_rcons cat_uniq {}IHn uniq_enum_normal_sz andbT /=.
+apply/negP => /hasP[/= u]; rewrite mem_enum_normalP => /andP[/eqP szu _].
+case/flattenP => /= l /trajectP[i ltin {l}->].
+rewrite mem_enum_normalP => /andP[ + _].
+by rewrite szu gtn_eqF.
+Qed.
+
 End EnumNormalForms.
+
+
+(* isopres preserve the number of normal forms (if finite) *)
+Section IsoCan.
+
+Context {Alph Beta : choiceType}
+  (P : pres Alph) (Q : pres Beta)
+  (Qconv : convergent (prelat Q))
+  (isoPQ : isopres P Q).
+
+Definition isocan u := normal_of Qconv.2 (isoPQ u).
+Local Lemma isocan_words w : w \in words_of P -> isocan w \in words_of Q.
+Proof.
+have [_ /rewrites_to_words_ofE <-] := normal_ofP Qconv.2 (isoPQ w).
+by move/(isopres_word_of isoPQ).
+Qed.
+Local Lemma isocanP u : normalf (prelat Q) (isoPQ u) (isocan u).
+Proof. exact: normal_ofP. Qed.
+
+End IsoCan.
+
+
+Section IsoCanK.
+
+Context {Alph Beta : choiceType}
+  (P : pres Alph) (Q : pres Beta)
+  (Pconv : convergent (prelat P))
+  (Qconv : convergent (prelat Q))
+  (isoPQ : isopres P Q).
+
+Let P2Q := isocan Qconv isoPQ.
+Let Q2P := isocan Pconv (isopres_sym isoPQ).
+
+Lemma isocanK u :
+  (u \in words_of P) && (normal (prelat P) u) -> Q2P (P2Q u) = u.
+Proof.
+case/andP => uinP norPu.
+have norfPu : normalf (prelat P) u u by split => //; apply: rewrites_to_refl.
+have /equiv_sym := canmor isoPQ uinP; rewrite -(normalf_equivE Pconv.1 norfPu).
+move/(confluentE Pconv.1 _); apply.
+rewrite (normalf_equivE Pconv.1 (isocanP Pconv (isopres_sym isoPQ) (P2Q u))).
+rewrite (isopres_invP _ (isocan_words _ _ uinP) (isopres_word_of _ uinP)).
+by have [_ /rewrites_to_equiv/equiv_sym] := isocanP Qconv isoPQ u.
+Qed.
+
+End IsoCanK.
+
+
+Section NormalIso.
+
+Context {Alph Beta : choiceType}
+  (P : pres Alph) (Q : pres Beta)
+  (Pconv : convergent (prelat P))
+  (Qconv : convergent (prelat Q))
+  (isoPQ : isopres P Q)
+  (lP : seq (word Alph)) (lQ : seq (word Beta))
+  (norlP :   is_enum_normal P lP) (norlQ : is_enum_normal Q lQ).
+
+Theorem isopres_perm_eq_enum : perm_eq [seq isocan Qconv isoPQ i | i <- lP] lQ.
+Proof.
+move: norlP norlQ; rewrite /is_enum_normal => -[uniqlP memlP] [uniqlQ memlQ].
+set P2Q := isocan Qconv isoPQ.
+pose Q2P := isocan Pconv (isopres_sym isoPQ).
+have P2QK : {in lP, cancel P2Q Q2P} by move=> u; rewrite -memlP; exact: isocanK.
+have Q2PK : {in lQ, cancel Q2P P2Q} by move=> v; rewrite -memlQ; exact: isocanK.
+apply: uniq_perm => //.
+  rewrite map_inj_in_uniq => //; first exact: (can_in_inj P2QK).
+move=> /= v; rewrite -memlQ; apply/mapP/idP => [[u]|].
+  rewrite -memlP => /andP[uinP _ {v}->].
+  rewrite (isocan_words _ _ uinP) /=.
+  by have[] := isocanP Qconv isoPQ u.
+case/andP => vinQ norv; exists (Q2P v).
+  rewrite -memlP; rewrite (isocan_words _ _ vinQ) /=.
+  by have[] := isocanP Pconv (isopres_sym isoPQ) v.
+by rewrite Q2PK // -memlQ vinQ norv.
+Qed.
+Corollary isopres_size_enum : size lP = size lQ.
+Proof. by have /perm_size := isopres_perm_eq_enum; rewrite size_map. Qed.
+
+End NormalIso.
+
